# 常用求和公式

[toc]

## $\sum_{i=1}^{n}i$

$$
\begin{aligned}\sum_{i=1}^{n}i=\frac{(n+1)n}{2} \end{aligned}
$$

## $\sum_{i=1}^{n}i^2$

$$
\begin{aligned} (n+1)^3-1=&\sum_{i=1}^{n}[(i+1)^3-i^3]\\=&\sum_{i=1}^{n}[3i^2+3i+1]\\=&3\sum_{i=1}^{n}i^2+3\frac{(n+1)n}{2}+n \end{aligned}
$$

$$
\begin{aligned} \sum_{i=1}^{n}i^2=&\frac{(n^3+3n^2+3n)}{3}-\frac{(n+1)n}{2}-\frac{n}{3}\\=&\frac{2n^3+3n^2+n}{6} \end{aligned}
$$

## $\sum_{i=1}^{n}i^3$

$$
\begin{aligned} (n+1)^4-1=&\sum_{i=1}^{n}[(i+1)^4-i^4]\\=&\sum_{i=1}^{n}[4i^3+6i^2+4i+1]\\=&4\sum_{i=1}^{n}i^3+6\frac{2n^3+3n^2+n}{6}+4\frac{(n+1)n}{2}+n \end{aligned}
$$

$$
\begin{aligned} \sum_{i=1}^{n}i^3=&\frac{(n^4+4n^3+6n^2+4n)}{4}-\frac{2n^3+3n^2+n}{4}-\frac{(n+1)n}{2}-\frac{n}{4}\\=&\frac{n^4+2n^3+n^2}{4} \end{aligned}
$$